MathematicalLogic/Equality/Theory.lean
@@ -17,7 +17,7 @@ def Terms.eq : Terms 𝓛 n → Terms 𝓛 n → Formula 𝓛
 infix:60 " ≋ " => Terms.eq
 
 def Formula.exists_unique (p : Formula 𝓛) :=
-  ∃' (p ⋀ ∀' (↑ₚp ⟶ #1 ≈ (#0 : Term 𝓛)))
+  ∃' (p ⋀ ∀' (↑ₚp ⇒ #1 ≈ (#0 : Term 𝓛)))
 prefix:max "∃'! " => Formula.exists_unique
 
 def BTerm.eq (t₁ t₂ : BTerm 𝓛 m) : BFormula 𝓛 m :=
@@ -33,7 +33,7 @@ def BTerms.eq : BTerms 𝓛 m n → BTerms 𝓛 m n → BFormula 𝓛 m
 infix:60 " ≋ᵇ " => BTerms.eq
 
 def BFormula.exists_unique (p : BFormula 𝓛 (m + 1)) :=
-  ∃ᵇ (p ⋀ ∀ᵇ (↑ₚᵇp ⟶ #ᵇ1 ≈ᵇ #ᵇ0))
+  ∃ᵇ (p ⋀ ∀ᵇ (↑ₚᵇp ⇒ #ᵇ1 ≈ᵇ #ᵇ0))
 prefix:max "∃ᵇ! " => BFormula.exists_unique
 
 @[simp] theorem Term.subst_eq {t₁ t₂ : Term 𝓛} : (t₁ ≈ t₂)[σ]ₚ = t₁[σ]ₜ ≈ t₂[σ]ₜ := by simp [Term.eq]
@@ -51,7 +51,7 @@ prefix:max "∃ᵇ! " => BFormula.exists_unique
 
 inductive EQ : Theory 𝓛 where
 | e1 : EQ (∀ᵇ (#ᵇ0 ≈ᵇ #ᵇ0))
-| e2 : EQ (∀* (t₁ ≈ᵇ t₂ ⟶ p[↦ᵇ t₁]ₚᵇ ⟶ p[↦ᵇ t₂]ₚᵇ))
+| e2 : EQ (∀* (t₁ ≈ᵇ t₂ ⇒ p[↦ᵇ t₁]ₚᵇ ⇒ p[↦ᵇ t₂]ₚᵇ))
 
 class EqTheory (𝓣 : Theory 𝓛) where
   eqAxioms : EQ ⊆ 𝓣
@@ -83,12 +83,12 @@ theorem refl_terms {ts : Terms 𝓛 n} : 𝓣 ⊢ ts ≋ ts :=
     · apply refl_terms
 
 theorem subst {t₁ t₂ : Term 𝓛} {p : Formula 𝓛} :
-  𝓣 ⊢ t₁ ≈ t₂ ⟶ p[↦ₛ t₁]ₚ ⟶ p[↦ₛ t₂]ₚ := by
+  𝓣 ⊢ t₁ ≈ t₂ ⇒ p[↦ₛ t₁]ₚ ⇒ p[↦ₛ t₂]ₚ := by
   let m := max p.bound (max t₁.bound t₂.bound)
   let t₁' := t₁.bounded (m := m) (by simp [m])
   let t₂' := t₂.bounded (m := m) (by simp [m])
   let p' := p.bounded (m := m + 1) (by simp [m, Nat.le_succ_of_le])
-  have h : 𝓣 ⊢ ∀* ((t₁' ≈ᵇ t₂') ⟶ p'[↦ᵇ t₁']ₚᵇ ⟶ p'[↦ᵇ t₂']ₚᵇ) := by
+  have h : 𝓣 ⊢ ∀* ((t₁' ≈ᵇ t₂') ⇒ p'[↦ᵇ t₁']ₚᵇ ⇒ p'[↦ᵇ t₂']ₚᵇ) := by
     apply Theory.axioms
     apply EqTheory.eqAxioms
     apply EQ.e2
@@ -98,7 +98,7 @@ theorem subst {t₁ t₂ : Term 𝓛} {p : Formula 𝓛} :
   exact h
 
 theorem symm {t₁ t₂ : Term 𝓛} :
-  𝓣 ⊢ t₁ ≈ t₂ ⟶ t₂ ≈ t₁ := by
+  𝓣 ⊢ t₁ ≈ t₂ ⇒ t₂ ≈ t₁ := by
   pintro
   have h := subst (𝓣 := 𝓣) (t₁ := t₁) (t₂ := t₂) (p := #0 ≈ ↑ₜt₁)
   simp [Term.shift_subst_single] at h
@@ -109,7 +109,7 @@ theorem symm {t₁ t₂ : Term 𝓛} :
 macro "psymm" : tactic => `(tactic| (apply mp (weaken (by pweaken_ctx) symm)))
 
 theorem symm_terms {ts₁ ts₂ : Terms 𝓛 n} :
-  𝓣 ⊢ ts₁ ≋ ts₂ ⟶ ts₂ ≋ ts₁ :=
+  𝓣 ⊢ ts₁ ≋ ts₂ ⇒ ts₂ ≋ ts₁ :=
   match ts₁, ts₂ with
   | []ₜ, []ₜ => Proof.identity
   | t₁ ∷ₜ ts₁, t₂ ∷ₜ ts₂ => by
@@ -123,7 +123,7 @@ theorem symm_terms {ts₁ ts₂ : Terms 𝓛 n} :
       passumption
 
 theorem trans {t₁ t₂ t₃ : Term 𝓛} :
-  𝓣 ⊢ t₁ ≈ t₂ ⟶ t₂ ≈ t₃ ⟶ t₁ ≈ t₃ := by
+  𝓣 ⊢ t₁ ≈ t₂ ⇒ t₂ ≈ t₃ ⇒ t₁ ≈ t₃ := by
   pintro
   have h := subst (𝓣 := 𝓣) (t₁ := t₂) (t₂ := t₁) (p := #0 ≈ ↑ₜt₃)
   simp [Term.shift_subst_single] at h
@@ -139,14 +139,14 @@ macro_rules
 | `(tactic| ptrans $t) => `(tactic| (apply mp2 (weaken (by pweaken_ctx) (trans (t₂ := $t)))))
 
 theorem subst_iff {t₁ t₂ : Term 𝓛} {p : Formula 𝓛} :
-  𝓣 ⊢ t₁ ≈ t₂ ⟶ (p[↦ₛ t₁]ₚ ⟷ p[↦ₛ t₂]ₚ) := by
+  𝓣 ⊢ t₁ ≈ t₂ ⇒ (p[↦ₛ t₁]ₚ ⇔ p[↦ₛ t₂]ₚ) := by
   pintro
   apply Proof.mp2 Proof.iff_intro <;> apply Proof.mp (Proof.weaken_add subst)
   · passumption
   · psymm; passumption
 
 theorem subst_term {t t₁ t₂ : Term 𝓛} :
-  𝓣 ⊢ t₁ ≈ t₂ ⟶ t[↦ₛ t₁]ₜ ≈ t[↦ₛ t₂]ₜ := by
+  𝓣 ⊢ t₁ ≈ t₂ ⇒ t[↦ₛ t₁]ₜ ≈ t[↦ₛ t₂]ₜ := by
   pintro
   have h := subst (𝓣 := 𝓣) (t₁ := t₁) (t₂ := t₂) (p := ↑ₜ(t[↦ₛ t₁]ₜ) ≈ t)
   simp [Term.shift_subst_single] at h
@@ -163,7 +163,7 @@ lemma cast_func {f : 𝓛.𝓕 n} {ts₁ : Terms 𝓛 n} {ts₂ : Terms 𝓛 m} 
 
 lemma congr_func_aux
   {f : 𝓛.𝓕 (n + m)} {ts₁ ts₂ : Terms 𝓛 n} {ts : Terms 𝓛 m} :
-  𝓣 ⊢ ts₁ ≋ ts₂ ⟶ f ⬝ₜ (ts ++ ts₁) ≈ f ⬝ₜ (ts ++ ts₂) :=
+  𝓣 ⊢ ts₁ ≋ ts₂ ⇒ f ⬝ₜ (ts ++ ts₁) ≈ f ⬝ₜ (ts ++ ts₂) :=
   match n, ts₁, ts₂ with
   | 0, []ₜ, []ₜ => by pintro; prefl
   | n + 1, t₁ ∷ₜ ts₁, t₂ ∷ₜ ts₂ => by
@@ -182,7 +182,7 @@ lemma congr_func_aux
       passumption
 
 theorem congr_func {f : 𝓛.𝓕 n} {ts₁ ts₂ : Terms 𝓛 n} :
-  𝓣 ⊢ ts₁ ≋ ts₂ ⟶ f ⬝ₜ ts₁ ≈ f ⬝ₜ ts₂ :=
+  𝓣 ⊢ ts₁ ≋ ts₂ ⇒ f ⬝ₜ ts₁ ≈ f ⬝ₜ ts₂ :=
   congr_func_aux (ts := []ₜ)
 
 lemma cast_atom {p : 𝓛.𝓟 n} {ts₁ : Terms 𝓛 n} {ts₂ : Terms 𝓛 m} (h : n = m) :
@@ -194,7 +194,7 @@ lemma cast_atom {p : 𝓛.𝓟 n} {ts₁ : Terms 𝓛 n} {ts₂ : Terms 𝓛 m} 
 
 lemma congr_atom_aux
   {p : 𝓛.𝓟 (n + m)} {ts₁ ts₂ : Terms 𝓛 n} {ts : Terms 𝓛 m} :
-  𝓣 ⊢ ts₁ ≋ ts₂ ⟶ p ⬝ₚ (ts ++ ts₁) ⟶ p ⬝ₚ (ts ++ ts₂) :=
+  𝓣 ⊢ ts₁ ≋ ts₂ ⇒ p ⬝ₚ (ts ++ ts₁) ⇒ p ⬝ₚ (ts ++ ts₂) :=
   match n, ts₁, ts₂ with
   | 0, []ₜ, []ₜ => by pintro; exact Proof.identity
   | n + 1, t₁ ∷ₜ ts₁, t₂ ∷ₜ ts₂ => by
@@ -213,11 +213,11 @@ lemma congr_atom_aux
       passumption
 
 theorem congr_atom {p : 𝓛.𝓟 n} {ts₁ ts₂ : Terms 𝓛 n} :
-  𝓣 ⊢ ts₁ ≋ ts₂ ⟶ p ⬝ₚ ts₁ ⟶ p ⬝ₚ ts₂ :=
+  𝓣 ⊢ ts₁ ≋ ts₂ ⇒ p ⬝ₚ ts₁ ⇒ p ⬝ₚ ts₂ :=
   congr_atom_aux (ts := []ₜ)
 
 theorem congr_atom_iff {p : 𝓛.𝓟 n} {ts₁ ts₂ : Terms 𝓛 n} :
-  𝓣 ⊢ ts₁ ≋ ts₂ ⟶ (p ⬝ₚ ts₁ ⟷ p ⬝ₚ ts₂) := by
+  𝓣 ⊢ ts₁ ≋ ts₂ ⇒ (p ⬝ₚ ts₁ ⇔ p ⬝ₚ ts₂) := by
   pintro
   apply Proof.mp2 Proof.iff_intro <;> apply Proof.mp (Proof.weaken_add congr_atom)
   · passumption
